src/compiler/core/Core_init.thy
@@ -284,10 +284,10 @@ definition "activate_simp_optimization = True"
 
 definition "bootstrap_floor f_x l env =
  (let (l, env) = f_x l env
-    ; l_setup = Isab_thy_ml_extended (ML_setup (SML_compiler_env_config (env \<lparr> D_output_disable_thy := True
-                                                              , D_output_header_thy := None
-                                                              , D_output_position := (0, 0) \<rparr>) ))
-            # l
+    ; l_setup = Isab_thy_setup_env (Boot_setup_env (env \<lparr> D_output_disable_thy := True
+                                                        , D_output_header_thy := None
+                                                        , D_output_position := (0, 0) \<rparr>) )
+                # l
     ; l = if case D_input_meta env of [] \<Rightarrow> True | x # _ \<Rightarrow> ignore_meta_header x then
             l
           else
@@ -295,7 +295,7 @@ definition "bootstrap_floor f_x l env =
   ( if D_output_auto_bootstrap env then
       l
     else
-      Isab_thy_generation_syntax (Gen_semantics (D_ocl_semantics env))
+      Isab_thy_generation_syntax (Boot_generation_syntax (D_ocl_semantics env))
       # l_setup
   , env \<lparr> D_output_auto_bootstrap := True \<rparr> ))"
 
